Slight refactor

fstar/MLS.TreeSync.Symbolic.LeafNodeSignature.fst
@@ -1,4 +1,4 @@
-module MLS.TreeSync.Symbolic.SignatureGuarantees
+module MLS.TreeSync.Symbolic.LeafNodeSignature
 
 open Comparse
 open MLS.Crypto
@@ -65,6 +65,9 @@ val tree_list_has_pred: tkp:treekem_parameters -> timestamp -> tree_list dy_byte
 let tree_list_has_pred tkp time tl =
   for_allP (tkp.pred time) tl
 
+val leaf_node_label: string
+let leaf_node_label = "LeafNodeTBS"
+
 val leaf_node_spred: treekem_parameters -> sign_pred
 let leaf_node_spred tkp usg time vk ln_tbs_bytes =
   match (parse (leaf_node_tbs_nt dy_bytes tkp.types) ln_tbs_bytes) with
@@ -83,6 +86,10 @@ let leaf_node_spred tkp usg time vk ln_tbs_bytes =
     | LNS_key_package () ->
       forall li. tkp.pred time (|0, li, TLeaf (Some ({data = ln_tbs.data; signature = empty #dy_bytes;} <: leaf_node_nt dy_bytes tkp.types))|)
   )
+
+val has_leaf_node_tbs_invariant: treekem_parameters -> global_usage -> prop
+let has_leaf_node_tbs_invariant tkp gu =
+  has_sign_pred gu leaf_node_label (leaf_node_spred tkp)
 
 (*** Proof for verification ***)
 
@@ -185,7 +192,7 @@ let rec leaf_at_has_pre #bytes #bl #tkt #l #i pre t li =
 #push-options "--z3rlimit 100"
 val parent_hash_implies_treekem_pred: #l:nat -> #i:tree_index l -> gu:global_usage -> time:timestamp -> tkp:treekem_parameters -> group_id:mls_bytes dy_bytes -> t:treesync dy_bytes tkp.types l i -> ast:as_tokens dy_bytes (dy_asp gu time).token_t l i -> Lemma
   (requires
-    has_sign_pred gu "LeafNodeTBS" (leaf_node_spred tkp) /\
+    has_leaf_node_tbs_invariant tkp gu /\
     unmerged_leaves_ok t /\ parent_hash_invariant t /\ valid_leaves_invariant group_id t /\
     node_not_blank t /\
     all_credentials_ok t ast /\
@@ -345,7 +352,7 @@ let external_path_has_pred #tkp #l #li time t p group_id sk nonce =
 #push-options "--z3rlimit 25"
 val is_valid_external_path_to_path: #tkp:treekem_parameters -> #l:nat -> #li:leaf_index l 0 -> gu:global_usage -> time:timestamp -> t:treesync dy_bytes tkp.types l 0 -> p:external_pathsync dy_bytes tkp.types l 0 li -> group_id:mls_bytes dy_bytes -> sk:sign_private_key dy_bytes -> nonce:sign_nonce dy_bytes -> Lemma
   (requires
-    has_sign_pred gu "LeafNodeTBS" (leaf_node_spred tkp) /\
+    has_leaf_node_tbs_invariant tkp gu /\
     treesync_has_pre (is_valid gu time) t /\
     external_pathsync_has_pre (is_valid gu time) p /\
     is_valid gu time group_id /\
